iris/UnionLinkInstAt.v
@@ -1,0 +1,206 @@
+(* ===================================================================== *)
+(*  UnionLinkInstAt.v -- THE UNION LINK RECORD AT A NAMED BOOT STATE      *)
+(*  (cut C9f1; design: claude-notes/design/union.md section 3, 'The       *)
+(*  credential the main loop carries').                                    *)
+(*                                                                        *)
+(*  [UnionLinkInst.union_link_inst] with the writer's witness pinned to   *)
+(*  the era's boot state [s0] -- [FileLinkGen.f0w_at] -- and the head at  *)
+(*  that state -- [FileLinksAt.fhead_at]: RULING H' of the file round     *)
+(*  ([FileLinkGen.file_link_gen_at]), at the union model.  The shell's    *)
+(*  round names [s0] and ties the deed to it by a SHARED INDEX, so every  *)
+(*  block the record hands back is at [s0] structurally.                   *)
+(*                                                                        *)
+(*  The one field that is not [file_link_gen_at]'s shape is the N-writer  *)
+(*  arm: [union_X_at s0] is [UnionLinkInst.union_X] beside a witness of   *)
+(*  the era's boot state [f0cw k s0], which is what turns the filing      *)
+(*  link's returned witness (at SOME boot state) into the record's (at    *)
+(*  [s0]).                                                                *)
+(* ===================================================================== *)
+From Stdlib Require Import ZArith Lia List.
+From stdpp Require Import gmap list bitvector.definitions.
+From iris.proofmode Require Import proofmode.
+From iris.base_logic.lib Require Import mono_nat own ghost_var ghost_map.
+From iris.algebra.lib Require Import mono_list.
+Require Import SailStdpp.Operators_mwords.
+Require Import SailStdpp.Base SailStdpp.TypeCasts SailStdpp.Values
+        SailStdpp.MachineWord.
+Require Import RiscvLang.
+Require Import ObsTrace.
+Require Import LineWords.
+Require Import EchoDisc.
+Require Import EchoOutPure.
+Require Import EchoOut.
+Require Import LineModel.
+Require Import LineModelLinks.
+Require Import GenOutPure.
+Require Import GenOut.
+Require Import AppEcho.
+Require Import FileState.
+Require Import FileDisc.
+Require Import AppFile.
+Require Import FileOut.
+Require Import FileLinksLine.
+Require Import FileLinksAt.       (* [fhead_at], [f0pre_at], [fturn_pre_at] *)
+Require Import FileLinkGen.       (* [f0w_at], [fhead_at_boot], [fhead_at_cur] *)
+Require Import PipeOut.
+Require Import ProgTree.
+Require Import PipesDisc.
+Require Import PipesView.
+Require Import PipeOutN.
+Require Import PipesLinksV.
+Require Import UnionDisc.
+Require Import UnionDiscDec.
+Require Import UnionView.
+Require Import UnionOut.
+Require Import UnionLinks.
+Require Import UnionLinkInst.
+Require Import GenLinksLine.
+Require Import LinkRec.
+Require Import RiscvPtsto.
+Require Import WpUart.
+From stdpp Require Import list.
+Local Open Scope list_scope.
+
+Local Notation U := ulmU.
+
+Section union_link_inst_at.
+  Context {Σ : gFunctors}.
+  Context `{!echoOutG Σ, !inG Σ (mono_listR (leibnizO Z)), !fileAppG Σ,
+            !fileOutG Σ, !pipeOutG Σ}.
+  Context (ug : union_gn).
+  Local Notation gf := (ugn_file ug).
+  Local Notation UT := (file_taint (fgn_cl gf)).
+  Local Notation UPIN := (era_pin (fgn_echo gf)).
+  Context `{HRg : !riscvGS Σ}.
+  Context `{GEN : GenId}.
+
+  (* =================================================================== *)
+  (*  1.  THE PARAMETERS AT [s0]                                          *)
+  (* =================================================================== *)
+  Lemma uf0w_at_bwk (s0 : fstate) (k : nat) (s : fstate) :
+    f0w_at gf s0 k s -∗ uf0bwk ug k s.
+  Proof using . iIntros "[H _]". iApply (uf0w_bwk ug with "H"). Qed.
+
+  Lemma uf0w_at_bwk0 (s0 : fstate) (k : nat) (s : fstate) :
+    f0w_at gf s0 k s -∗ uf0bwk ug (S gen_id) s.
+  Proof using . iIntros "[H _]". iApply (uf0w_bwk0 ug with "H"). Qed.
+
+  Definition union_params_at (s0 : fstate) : gen_params U :=
+    MkGP U ulmU_laws ulmU_hooks
+      UT _ _
+      UPIN _ _ (era_pin_agree (fgn_echo gf))
+      (f0w_at gf s0) _ _
+      (uf0bwk ug) _ _ (S gen_id) (uf0w_at_bwk s0) (uf0w_at_bwk0 s0) (uf0bwk_agree ug)
+      (fhead_at gf s0) _ (fhead_at_cur gf s0) (fhead_at_inp gf s0).
+
+  Lemma union_params_at_T (s0 : fstate) : gT (union_params_at s0) = UT.
+  Proof using . reflexivity. Qed.
+  Lemma union_params_at_PIN (s0 : fstate) : gPIN (union_params_at s0) = UPIN.
+  Proof using . reflexivity. Qed.
+  Lemma union_params_at_W (s0 : fstate) : gW (union_params_at s0) = f0w_at gf s0.
+  Proof using . reflexivity. Qed.
+
+  (* the links entail the interface at [s0] *)
+  Lemma union_links_gl_at (s0 : fstate) : union_links ug -∗ glinks U (union_params_at s0).
+  Proof using .
+    iIntros "Hlk". iDestruct (union_links_eq with "Hlk") as %Hc.
+    iApply (peclV_glinks (ugn_pipe ug) U (ucparams ug) (ulm_byte_laws adm_u_f) None
+              (uwa ug) Hc (union_params_at s0) eq_refl eq_refl (f0w_at_cw gf s0)
+              (or_introl I) (fhead_at_boot gf s0)).
+  Qed.
+
+  Lemma union_links_gl_w_at (s0 : fstate) : union_links ug -∗ gl_w U (union_params_at s0).
+  Proof using .
+    iIntros "Hlk". iDestruct (union_links_gl_at s0 with "Hlk") as "(H & _)". iExact "H".
+  Qed.
+  Lemma union_links_gl_blk_at (s0 : fstate) : union_links ug -∗ gl_blk U (union_params_at s0).
+  Proof using .
+    iIntros "Hlk". iDestruct (union_links_gl_at s0 with "Hlk") as "(_ & H & _)". iExact "H".
+  Qed.
+  Lemma union_links_gl_taint_at (s0 : fstate) :
+    union_links ug -∗ gl_taint U (union_params_at s0).
+  Proof using .
+    iIntros "Hlk". iDestruct (union_links_gl_at s0 with "Hlk") as "(_ & _ & _ & _ & H)".
+    iExact "H".
+  Qed.
+
+  (* =================================================================== *)
+  (*  2.  THE TURN AND THE RESIDUE                                        *)
+  (* =================================================================== *)
+  Lemma uturn0_at (s0 : fstate) (k : nat) :
+    fturn_pre_at gf s0 k -∗
+    (∃ v : era_pins, UPIN k v ∗ dl_cnt v (1/2) 0%nat ∗ inp_lb v [])
+    ∗ (∃ v : era_pins, UPIN k v ∗ gwc_ban U (union_params_at s0) k v [] 0%nat).
+  Proof using .
+    rewrite /fturn_pre_at /FileOut.fturn_core.
+    iIntros "(%Hk & Ht & Hpre)".
+    iDestruct "Ht" as (v vf) "(#Hpin & #Hvf & Htn & Hdl & #Hcs & #Hps & #HE)".
+    iSplitL "Hdl"; [iExists v; by iFrame "Hpin Hdl HE" |].
+    iExists v. iFrame "Hpin". rewrite /gwc_ban. iRight. iLeft.
+    iSplitR; [by iPureIntro |]. rewrite /gH /union_params_at /fhead_at.
+    iSplitR; [by iPureIntro |]. iSplitR; [by iPureIntro |].
+    iFrame "Htn Hps Hcs HE Hpre". iExists vf. iExact "Hvf".
+  Qed.
+
+  (* the residue is the unindexed record's: the reader's witness is the
+     same at both parameter records *)
+  Lemma urresw_res_at (s0 : fstate) (v : era_pins) (I : list (bv 8)) :
+    urresw ug v I -∗ gwc_rres U (union_params_at s0) v I.
+  Proof using . rewrite /urresw /gwc_rres. iIntros "[$ _]". Qed.
+
+  (* =================================================================== *)
+  (*  3.  THE N-WRITER ARM AT [s0]                                        *)
+  (* =================================================================== *)
+  Definition union_X_at (s0 : fstate) (k : nat) (v : era_pins) (I : list (bv 8))
+      : iProp Σ :=
+    (union_X ug k v I ∗ f0cw gf k s0)%I.
+
+  Global Instance union_X_at_timeless s0 k v I : Timeless (union_X_at s0 k v I).
+  Proof using .
+    rewrite /union_X_at. apply bi.sep_timeless; [apply union_X_timeless | apply _].
+  Qed.
+
+  Lemma union_X_dollar_at (s0 : fstate) (k : nat) (v : era_pins) (I : list (bv 8))
+      (b : bv 8) (Φ : iProp Σ) :
+    b = u_prompt !!! 0%nat ->
+    UPIN k v -∗ union_links ug -∗ union_X_at s0 k v I -∗
+    (gwc_sp_t U (union_params_at s0) k v I -∗ Φ) -∗ out_link Uart0 k b Φ.
+  Proof using .
+    intros Hb. iIntros "#Hpin #Hlk [Hx #Hw0] HΦ".
+    iApply (union_X_dollar ug k v I b Φ Hb with "Hpin Hlk Hx").
+    iIntros "Hsp". iApply "HΦ". rewrite /gwc_sp_t.
+    iDestruct "Hsp" as "[Hx | #HT]"; [| by iRight].
+    iDestruct "Hx" as (ps cs s P) "[%Hw Hc]". iLeft. iExists ps, cs, s, P.
+    iSplitR; [by iPureIntro |]. rewrite /gcur.
+    iDestruct "Hc" as "(Htn & Hps & Hcs & HE & #HW)". iFrame "Htn Hps Hcs HE".
+    cbn [gW union_params union_params_at]. rewrite /f0w_at.
+    iAssert (⌜s = s0⌝)%I as %->.
+    { rewrite /f0w /f0cw. iDestruct "HW" as "[_ HW]".
+      iDestruct "HW" as (vf) "[#Hvf #Hlb]". iDestruct "Hw0" as (vf') "[#Hvf' #Hlb']".
+      iDestruct (file_era_pin_agree with "Hvf Hvf'") as %<-.
+      iApply (f0_lb_agree with "Hlb Hlb'"). }
+    iSplitL; [iExact "HW" | done].
+  Qed.
+
+  (* =================================================================== *)
+  (*  4.  THE RECORD                                                      *)
+  (* =================================================================== *)
+  Definition union_link_inst_at (s0 : fstate) : LinkRec Σ :=
+    gen_link_inst U (union_params_at s0) (union_X_at s0) (union_X_at_timeless s0)
+      (union_links ug) (union_links_persistent ug) (union_links_gl_at s0)
+      (union_X_dollar_at s0) (uread_ret ug) (uread_ret_res ug) (fturn_pre_at gf s0)
+      (uturn0_at s0) (urresw ug) (urresw_persistent ug) (urresw_timeless ug)
+      (urresw_res_at s0) (ualt_code (UR RFSilent)).
+
+  Lemma union_at_T (s0 : fstate) : lk_T (union_link_inst_at s0) = UT.
+  Proof using . reflexivity. Qed.
+  Lemma union_at_pin (s0 : fstate) : lk_pin (union_link_inst_at s0) = UPIN.
+  Proof using . reflexivity. Qed.
+  Lemma union_at_links (s0 : fstate) : lk_links (union_link_inst_at s0) = union_links ug.
+  Proof using . reflexivity. Qed.
+  Lemma union_at_rres (s0 : fstate) : lk_rres (union_link_inst_at s0) = urresw ug.
+  Proof using . reflexivity. Qed.
+  Lemma union_at_lpr (s0 : fstate) :
+    lk_lpr (union_link_inst_at s0) = gwc_lpr U (union_params_at s0) (union_X_at s0).
+  Proof using . reflexivity. Qed.
+End union_link_inst_at.
